\section{Fonction d√©finie par morceaux}
\vspace{-2.5\baselineskip}
\begin{gather*}
f(t) = \left\{ \begin{array}{cc}
 0 & t < \pi \\
 f(t) & t \geq \pi
  \end{array}
  \right.
\;\;\Longleftrightarrow\;\; f(t)u(t-\pi)
\end{gather*}\vspace{-\baselineskip}\\
Inverse (exemple):
\begin{align*}
 y(t)   =&\; (e^{-3t}+e^t)u(t)\tag{1}\\
        &\quad+\frac{1}{4}(e^{t-1}-e^{-3t+3})u(t-1)\tag{2}\\
        &\qquad-\frac{1}{4}(e^{t-2}-e^{-3t+6})u(t-2)\tag{3}
\end{align*}
\begin{equation*}
y(t) = \left\{ \begin{array}{cc}
 0 & t < 0 \\
 (1) & 0\leq t<1\\
 (1)+(2) & 1\leq t<2\\
 (1)+(2)+(3) & t\geq 2
  \end{array}
  \right.
\end{equation*}

\subsubsection{TI}
\centering
\(f(t)\:\mathbf{step}(t-a)\)\\\raggedright